\section{Normal Sampling}
\subsection*{Task A}
\begin{theorem}\label{thm:invertgauss}
	Let $X$ be a continuous real-valued random variable with CDF $F_X:\mathbb{R}\to [0,1]$.
	Assume that $F_X$ is invertible. Then the random variable $Y:=F_X(X) \in [0,1]$ is uniformly distributed in $[0,1]$.
\end{theorem}
\begin{proof}
	We know that the CDF of a $\textrm{Uniform}[0,1]$ random variable is given by $F_X(x) = x$ for $0\leq x\leq 1$.
	To show that $Y$ is uniform on $[0, 1]$, we need to show that the CDF of $Y$ is $F_Y(u) = u$ for $0 \leq u \leq 1$.
	\begin{align*}
		F_Y(u) & = P\left\{Y \leq u\right\}           \\
		       & = P\left\{F_X(X) \leq u\right\}      \\
		       & = P\left\{X \leq F_X^{-1}(u)\right\} \\
		       & = F_X\left(F_X^{-1}(u)\right)        \\
		       & = u
	\end{align*}
	This shows that $Y \sim \textrm{Uniform}[0,1]$.
\end{proof}

\subsection*{Task B}
Consider $X \sim \mathcal{N}(0,1)$ and let $F_X$ be the CDF of $X$, and $f_X$ be the PDF of $X$.
\begin{align*}
	f_X(x) = \frac{1}{\sqrt{2\pi}}e^{-\frac{x^2}{2}}
\end{align*}
According to the problem statement, we need to formulate an algorithm $\cal{A}$ that generates a random variable with CDF and PDF equal to that of $X$, using only uniform random variables.

\begin{algorithm}
	\caption{$\cal{A}$: Obtaining Gaussian Distribution from a Uniform Distribution}
	\begin{algorithmic}
		\State Sample $y \sim Y$
		\State Compute $x \gets F_X^{-1}(y)$
		\State return $x$
	\end{algorithmic}
\end{algorithm}

\begin{claim}
	$F_X$ is strictly increasing, and hence invertible.
\end{claim}
\begin{proof}
	The derivative of $F_X(x)$ is given by $f_X(x)$, which is strictly positive for all $x$. Hence, $F_X$ is strictly increasing and hence invertible.
\end{proof}

\begin{claim}
	The distribution generated by algorithm $\cal{A}$ is equal to that of $X$, i.e., $F_{\cal{A}} (u) = F_X(u)$.
\end{claim}
\begin{proof}
	We start by noting that algorithm $\cal{A}$ essentially gives us the random variable $F_X^{-1}(Y)$.
	Since $X$ is a continuous real-valued random variable and $F_X$ is invertible, then from \cref{thm:invertgauss}, we know that if $Z := F_X(X)$, then $Z$ is uniform on $[0,1]$.
	But, $Y$ is also uniform on $[0,1]$. Hence, $Y=Z$.
	\begin{align*}
		Y              & = Z = F_X(X)                                                             \\
		F_X^{-1}(Y)    & = F_X^{-1}(F_X(X)) = X                                                   \\
		F_{\cal{A}}(u) & = P\left\{F_X^{-1}(Y) \leq u\right\} = P\left\{X \leq u\right\} = F_X(u)
	\end{align*}
	This completes the proof for our claim.
\end{proof}

